IMP-/AExp.thy
@@ -6,7 +6,13 @@ We define non-nested arithmetic expressions on natural numbers.
 The defined operations are addition and modified subtraction. Based on the AExp theory of IMP.
 \<close>
 
-theory AExp imports Main begin
+theory AExp
+  imports
+    Main
+    "HOL-Library.Char_ord"
+    "HOL-Library.List_Lexorder"
+    "HOL-Library.Product_Lexorder"
+begin
 
 type_synonym vname = string
 type_synonym val = nat
@@ -16,49 +22,49 @@ text "Defining atomic expressions:"
 datatype atomExp = N val | V vname
 
 fun atomVal :: "atomExp \<Rightarrow> state \<Rightarrow> val" where
-"atomVal (V var) s = s var"|
-"atomVal (N number) _ = number"
+  "atomVal (V var) s = s var"|
+  "atomVal (N number) _ = number"
 
 text "Defining arithmetic operators and general form of expressions: "
 
 datatype aexp =  A atomExp            |
-                 Plus atomExp atomExp |
-                 Sub atomExp atomExp  | 
-                 Parity atomExp       |
-                 RightShift atomExp
+  Plus atomExp atomExp |
+  Sub atomExp atomExp  |
+  Parity atomExp       |
+  RightShift atomExp
 
 bundle aexp_syntax
 begin
 notation Plus            ("_ \<oplus> _" [60,60] 60) and
-         Sub             ("_ \<ominus> _" [60,60] 60) and
-         Parity          ("_ \<doteq>1" [60] 60)   and
-         RightShift      ("_\<then>" [60] 60)
+  Sub             ("_ \<ominus> _" [60,60] 60) and
+  Parity          ("_ \<doteq>1" [60] 60)   and
+  RightShift      ("_\<then>" [60] 60)
 
 end
 bundle no_aexp_syntax
 begin
 notation Plus            ("_ \<oplus> _" [60,60] 60) and
-         Sub             ("_ \<ominus> _" [60,60] 60) and
-         Parity          ("_ \<doteq>1" [60] 60)    and
-         RightShift      ("_\<then>" [60] 60)
+  Sub             ("_ \<ominus> _" [60,60] 60) and
+  Parity          ("_ \<doteq>1" [60] 60)    and
+  RightShift      ("_\<then>" [60] 60)
 end
 unbundle aexp_syntax
 
 fun aval :: "aexp \<Rightarrow> state \<Rightarrow> val" where
-"aval (A atomExp) s = atomVal atomExp s"        |
-"aval (a \<oplus> b) s = atomVal a s  + atomVal b s" |
-"aval (a \<ominus> b) s = atomVal a s - atomVal b s"  |
-"aval (a \<doteq>1) s = atomVal a s  mod 2"        |
-"aval (a \<then>) s = atomVal a s div 2"
+  "aval (A atomExp) s = atomVal atomExp s"        |
+  "aval (a \<oplus> b) s = atomVal a s  + atomVal b s" |
+  "aval (a \<ominus> b) s = atomVal a s - atomVal b s"  |
+  "aval (a \<doteq>1) s = atomVal a s  mod 2"        |
+  "aval (a \<then>) s = atomVal a s div 2"
 
 text "evaluation examples:"
 value "aval (V ''x'' \<oplus> N 5)  (\<lambda>x. if x = ''x'' then 7 else 0)"
 value "aval (V ''x'' \<ominus> N 5)  ((\<lambda>x. 0) (''x'':= 7))"
 
-text "Syntactic sugar to write states:"     
+text "Syntactic sugar to write states:"
 definition null_state ("<>") where
   "null_state \<equiv> \<lambda>x. 0"
-syntax 
+syntax
   "_State" :: "updbinds => 'a" ("<_>")
 translations
   "_State ms" == "_Update <> ms"
@@ -79,5 +85,74 @@ lemma "<a := 1, b := 2> = (<> (a := 1)) (b := (2::int))"
 
 value "aval (V ''x'' \<ominus> N 5) <''x'' := 7>"
 value "aval (V ''x'' \<ominus> N 10) <''x'' := 7>"
+
+
+instantiation atomExp :: order_bot
+begin
+
+fun less_eq_atomExp :: "atomExp \<Rightarrow> atomExp \<Rightarrow> bool" where
+  "less_eq_atomExp (N n1) (N n2) \<longleftrightarrow> n1 \<le> n2"
+| "less_eq_atomExp (V v1) (V v2) \<longleftrightarrow> v1 \<le> v2"
+| "less_eq_atomExp (N _) _ \<longleftrightarrow> True"
+| "less_eq_atomExp (V _) _ \<longleftrightarrow> False"
+
+definition less_atomExp :: "atomExp \<Rightarrow> atomExp \<Rightarrow> bool" where
+  "less_atomExp c1 c2 = (c1 \<le> c2 \<and> \<not> c2 \<le> c1)"
+
+definition bot_atomExp :: "atomExp" where
+  "bot_atomExp = N 0"
+
+instance
+proof(standard, goal_cases)
+  case 1 show ?case by (simp add: less_atomExp_def)
+next
+  case 2 show ?case using less_eq_atomExp.simps by (fast elim: less_eq_atomExp.elims)
+next
+  case 3 thus ?case by (fastforce elim: less_eq_atomExp.elims)
+next
+  case 4 thus ?case by (fastforce elim: less_eq_atomExp.elims)
+next
+  case 5 show ?case unfolding bot_atomExp_def using less_eq_atomExp.elims(3) by blast
+qed
+end
+
+instantiation aexp :: order_bot
+begin
+
+fun less_eq_aexp :: "aexp \<Rightarrow> aexp \<Rightarrow> bool" where
+  "less_eq_aexp (A a1) (A a2) \<longleftrightarrow> a1 \<le> a2"
+| "less_eq_aexp (Plus a1 a2) (Plus b1 b2) \<longleftrightarrow> (a1, a2) \<le> (b1, b2)"
+| "less_eq_aexp (Sub a1 a2) (Sub b1 b2) \<longleftrightarrow> (a1, a2) \<le> (b1, b2)"
+| "less_eq_aexp (Parity p1) (Parity p2) \<longleftrightarrow> p1 \<le> p2"
+| "less_eq_aexp (RightShift sh1) (RightShift sh2) \<longleftrightarrow> sh1 \<le> sh2"
+| "less_eq_aexp (A _) _ \<longleftrightarrow> True"
+| "less_eq_aexp _ (A _) \<longleftrightarrow> False"
+| "less_eq_aexp (Plus _ _) _ \<longleftrightarrow> True"
+| "less_eq_aexp _ (Plus _ _) \<longleftrightarrow> False"
+| "less_eq_aexp (Sub _ _) _ \<longleftrightarrow> True"
+| "less_eq_aexp _ (Sub _ _) \<longleftrightarrow> False"
+| "less_eq_aexp (Parity _) _ \<longleftrightarrow> True"
+| "less_eq_aexp _ (Parity _) \<longleftrightarrow> False"
+
+definition less_aexp :: "aexp \<Rightarrow> aexp \<Rightarrow> bool" where
+  "less_aexp c1 c2 = (c1 \<le> c2 \<and> \<not> c2 \<le> c1)"
+
+definition bot_aexp :: "aexp" where
+  "bot_aexp = A bot"
+
+instance
+proof(standard, goal_cases)
+  case 1 show ?case by (simp add: less_aexp_def)
+next
+  case (2 x) show ?case by(cases x; simp)
+next
+  case (3 x y z) thus ?case by (cases x; cases y; cases z) auto
+next
+  case (4 x y) thus ?case by (cases x; cases y) auto
+next
+  case 5 show ?case
+    unfolding bot_aexp_def using bot_atomExp_def less_eq_aexp.elims(3) by fastforce
+qed
+end
 
 end
