IMP-/Com.thy
@@ -2,7 +2,14 @@
 
 section "IMP- A reduced imperative language"
 
-theory Com imports Main AExp begin
+theory Com
+  imports
+    Main
+    AExp
+    "HOL-Library.Char_ord"
+    "HOL-Library.List_Lexorder"
+    "HOL-Library.Product_Lexorder"
+begin
 
 paragraph "Summary"
 text\<open>Syntax definition for IMP-. Based on the syntax definition of IMP\<close>
@@ -31,5 +38,45 @@ no_notation Assign ("_ ::= _" [1000, 61] 61) and
 end
 
 unbundle com_syntax
+
+instantiation com :: order_bot
+begin
+
+fun less_eq_com :: "com \<Rightarrow> com \<Rightarrow> bool" where
+  "less_eq_com (Assign v1 e1) (Assign v2 e2) \<longleftrightarrow> v1 \<le> v2 \<and> e1 \<le> e2"
+| "less_eq_com (Seq c1 c2) (Seq c3 c4) \<longleftrightarrow> less_eq_com c1 c3 \<and> less_eq_com c2 c4"
+| "less_eq_com (If v1 c1 c2) (If v2 c3 c4) \<longleftrightarrow> v1 \<le> v2 \<and> less_eq_com c1 c3 \<and> less_eq_com c2 c4"
+| "less_eq_com (While v1 c1) (While v2 c2) \<longleftrightarrow> v1 \<le> v2 \<and> less_eq_com c1 c2"
+| "less_eq_com SKIP _ \<longleftrightarrow> True"
+| "less_eq_com _ SKIP \<longleftrightarrow> False"
+| "less_eq_com (Assign _ _) _ \<longleftrightarrow> True"
+| "less_eq_com _ (Assign _ _) \<longleftrightarrow> False"
+| "less_eq_com (Seq _ _) _ \<longleftrightarrow> True"
+| "less_eq_com _ (Seq _ _) \<longleftrightarrow> False"
+| "less_eq_com (If _ _ _) _ \<longleftrightarrow> True"
+| "less_eq_com _ (If _ _ _) \<longleftrightarrow> False"
+
+definition less_com :: "com \<Rightarrow> com \<Rightarrow> bool" where
+  "less_com c1 c2 = (c1 \<le> c2 \<and> \<not> c2 \<le> c1)"
+
+definition bot_com :: "com" where
+  "bot_com = SKIP"
+
+instance
+proof(standard, goal_cases)
+  case 1 show ?case by (simp add: less_com_def)
+next
+  case (2 x) show ?case by(induction x; simp)
+next
+  case (3 x y z) thus ?case
+    by(induction x z arbitrary: y rule: less_eq_com.induct; auto; force elim: less_eq_com.elims)
+next
+  case (4 x y) thus ?case
+    by(induction x y rule: less_eq_com.induct; force elim: less_eq_com.elims)
+next
+  case 5 show ?case
+    unfolding bot_com_def by simp
+qed
+end
 
 end
